exists_code.mp

src/rpartrec.lean
@@ -21,7 +21,7 @@ inductive rpartrec (o : ℕ →. ℕ) : (ℕ →. ℕ) → Prop
 | prec {f g} : rpartrec f → rpartrec g → rpartrec (unpaired (λ a n,
     n.elim (f a) (λ y IH, do i ← IH, g (mkpair a (mkpair y i)))))
 | rfind {f} : rpartrec f → rpartrec (λ a, rfind (λ n, (λ m, m = 0) <$> f (mkpair a n)))
-| univn {f : ℕ →. ℕ} [decidable_pred f.dom] : rpartrec f → rpartrec (unpaired $ λ a n, 
+| univn {f : ℕ →. ℕ} {D : decidable_pred f.dom} : rpartrec f → rpartrec (unpaired $ λ a n, 
     nat.rpartrec.code.evaln a.unpair.1 f.eval_opt (of_nat _ a.unpair.2) n)
 
 namespace rpartrec
@@ -122,4 +122,241 @@ theorem nat_elim {f : α → ℕ} {g : α →. σ} {h : α × ℕ × σ →. σ}
   simp [encodek]
 end
 
+@[refl] theorem refl {f : α →. β} : f partrec_in f := nat.rpartrec.refl
+theorem refl_in (f : α →. β) : f partrec_in f := nat.rpartrec.refl
+
+@[trans] theorem trans {f : α →. σ} {g : β →. τ} {h : γ →. μ} : f partrec_in g → g partrec_in h → f partrec_in h :=
+nat.rpartrec.trans
+
+theorem nat_iff {f g} : f partrec_in g ↔ nat.rpartrec.reducible f g  :=
+by simp[rpartrec, encodable.encode, map]
+
+theorem bind {f : α →. β} {g : α × β →. σ} {h : γ →. τ}
+  (hf : f partrec_in h) (hg : g partrec_in h) : (λ a, (f a).bind (λ x, g (a, x))) partrec_in h :=
+(nat.rpartrec.comp hg (nat.rpartrec.some.pair hf)).of_eq $
+λ n, by simp [(<*>)]; cases e : decode α n with a;
+  simp [e, encodek]
+
+theorem map {f : α →. β} {g : α × β → σ} {h : γ →. τ}
+  (hf : f partrec_in h) (hg : (g : α × β →. σ) partrec_in h) : (λ a, (f a).map (λ x, g (a, x))) partrec_in h :=
+by simpa [bind_some_eq_map] 
+  using @rpartrec.bind _ _ _ _ _ _ _ _ _ _ _ (λ x, roption.some (g x)) _ hf hg
+
+theorem rfind {p : α × ℕ →. bool} : (λ a, nat.rfind (λ x, p (a, x))) partrec_in p :=
+  have c₀ : (λ x, (p x).map (λ b, cond b 0 1) : α × ℕ →. ℕ) partrec_in p :=
+    rpartrec.refl.map ((
+      (primrec.dom_bool (λ b, cond b 0 1)).comp primrec.snd).to_comp.to_rpart),
+((nat.rpartrec.rfind c₀).of_eq $ λ n, by 
+{ cases e : decode α n with a;
+  simp [e, nat.rfind_zero_none, map_id'],
+  congr, funext n,
+  simp [roption.map_map, (∘)],
+  apply map_id' (λ b, _),
+  cases b; refl })
+
 end rpartrec
+
+namespace rcomputable
+
+variables {α : Type*} {β : Type*} {γ : Type*} {σ : Type*} {τ : Type*} {μ : Type*}
+variables [primcodable α] [primcodable β] [primcodable γ] [primcodable σ] [primcodable τ] [primcodable μ]
+
+theorem of_eq {f g : α → σ} {h : β →. τ} (hf : f computable_in h) (H : ∀ n, f n = g n) :
+  g computable_in h := (funext H : f = g) ▸ hf
+
+theorem comp {f : β → γ} {g : α → β} {h : σ →. τ} 
+  (hf : f computable_in h) (hg : g computable_in h) : (λ a, f (g a)) computable_in h :=
+(nat.rpartrec.comp hf hg).of_eq $ λ n, by simp; cases e : decode α n with a; simp [e, encodek]
+
+theorem nat_elim
+  {f : α → ℕ} {g : α → σ} {h : α × ℕ × σ → σ} {o : β →. γ}
+  (hf : f computable_in o) (hg : g computable_in o) (hh : h computable_in o) :
+  (λ a, (f a).elim (g a) (λ y IH, h (a, y, IH))) computable_in o :=
+((rpartrec.nat_elim hf hg hh).of_eq) $
+λ a, by { unfold_coes, simp, induction f a with m, simp, simp[ih] }
+
+theorem id {f : β →. σ} : (@id α) computable_in f := computable.id.to_rcomp
+
+theorem fst {f : γ →. σ} : (@prod.fst α β) computable_in f := computable.fst.to_rcomp
+
+theorem snd {f : γ →. σ} : (@prod.snd α β) computable_in f := computable.snd.to_rcomp
+
+theorem pair {f : α → σ} {g : α → τ} {h : γ →. μ}
+  (hf : f computable_in h) (hg : g computable_in h) : (λ x, (f x, g x)) computable_in h
+:= (nat.rpartrec.pair hf hg).of_eq $ λ n, by cases decode α n; simp [(<*>)]
+
+theorem const (a : α) {f : γ →. σ} : (λ x, a : β → α) computable_in f :=
+(computable.const a).to_rcomp
+
+protected theorem encode {f : β →. σ} : (@encode α _) computable_in f := computable.encode.to_rcomp
+
+protected theorem decode {f : β →. σ} : (@decode α _) computable_in f := computable.decode.to_rcomp
+
+@[refl] theorem refl {f : α → β} : f computable_in (f : α →. β) := nat.rpartrec.refl
+theorem refl_in (f : α → β) : f computable_in (f : α →. β) := nat.rpartrec.refl
+
+@[trans] theorem trans {f : α → σ} {g : β → τ} {h : γ →. μ} :
+  f computable_in (g : β →. τ)→ g computable_in h → f computable_in h := nat.rpartrec.trans
+
+end rcomputable
+
+namespace nat.rpartrec.code
+open nat.rpartrec (code)
+
+private lemma evaln_comp' {c f} {g : ℕ → option ℕ} (h : eval f c = (λ x, g x)) : ∀ m, ∃ s₀,
+  ∀ n a, n < m → g n = some a → evaln s₀ f c n = some a := λ m,
+begin
+  induction m with m0 ih, simp,
+  rcases ih with ⟨s₀, hs₀⟩,
+  cases e : g m0 with v,
+  { refine ⟨s₀, λ n a en ha, _⟩,
+    have : n < m0 ∨ n = m0, from nat.lt_succ_iff_lt_or_eq.mp en,
+    cases this, { exact hs₀ _ _ this ha },
+    { exfalso, rw this at ha, rw e at ha, exact option.not_mem_none a ha } },
+  { unfold_coes at h,
+    have : v ∈ eval f c m0, simp[h, e],
+    have : ∃ k, v ∈ evaln k f c m0 := evaln_complete.mp this, rcases this with ⟨s₁, hs₁⟩,
+    refine ⟨max s₀ s₁, _⟩,
+    intros n a en ha,
+    have en' : n < m0 ∨ n = m0, from nat.lt_succ_iff_lt_or_eq.mp en,
+    cases en', 
+    { have : evaln s₀ f c n = option.some a := hs₀ _ _ en' ha,
+      show evaln (max s₀ s₁) f c n = option.some a,
+        from evaln_mono (le_max_left s₀ s₁) this },
+    { rw en', 
+      have : a = v, from option.some_inj.mp (by simp only [←e, ←ha, en']),
+      show evaln (max s₀ s₁) f c m0 = option.some a, rw this,
+        from evaln_mono (le_max_right s₀ s₁) hs₁ } }
+end
+
+@[simp] lemma eval_eval_opt {α β} (f : α →. β) [D : decidable_pred f.dom] {x} :
+  f.eval_opt x = @roption.to_option _ (f x) (D x) := rfl
+
+lemma eq_none_or_eq_some_dec {α} (o : roption α) [decidable o.dom] : o = none ∨ ∃ x, o = some x :=
+by { exact eq_none_or_eq_some o }
+
+--private lemma evaln_comp_dec {c f} [D : decidable_pred (eval f c).dom] : ∀ m, ∃ s₀,
+--  ∀ n a, n < m → eval f c n = some a → evaln s₀ f c n = some a := λ m,
+--begin
+--  induction m with m0 ih, simp,
+--  rcases ih with ⟨s₀, hs₀⟩,
+--  have e : eval f c m0 = none ∨ ∃ v, eval f c m0 = some v := eq_none_or_eq_some (eval f c m0),
+--  cases e,
+--  { refine ⟨s₀, λ n a en ha, _⟩,
+--    have : n < m0 ∨ n = m0, from nat.lt_succ_iff_lt_or_eq.mp en,
+--    cases this, { exact hs₀ _ _ this ha },
+--    { exfalso, rw this at ha, rw e at ha, exact roption.some_ne_none _ (eq.symm ha) } },
+--  { rcases e with ⟨v, e⟩,
+--    have : v ∈ eval f c m0, simp[e],
+--    have : ∃ k, v ∈ evaln k f c m0 := evaln_complete.mp this, rcases this with ⟨s₁, hs₁⟩,
+--    refine ⟨max s₀ s₁, _⟩,
+--    intros n a en ha,
+--    have en' : n < m0 ∨ n = m0, from nat.lt_succ_iff_lt_or_eq.mp en,
+--    cases en', 
+--    { have : evaln s₀ f c n = option.some a := hs₀ _ _ en' ha,
+--      show evaln (max s₀ s₁) f c n = option.some a,
+--        from evaln_mono (le_max_left s₀ s₁) this },
+--    { rw en', 
+--      have : a = v, from roption.some_inj.mp (by simp only [←e, ←ha, en']),
+--      show evaln (max s₀ s₁) f c m0 = option.some a, rw this,
+--        from evaln_mono (le_max_right s₀ s₁) hs₁ } }
+--end
+
+@[simp] theorem mem_to_option' {α} {o : roption α} [decidable o.dom] {a : α} :
+  to_option o = some a ↔ a ∈ o := mem_to_option
+
+--theorem eval_univn_eq_dec (c f) [D : decidable_pred (eval f c).dom] : 
+--  eval f c.univn = nat.unpaired (λ a n, (evaln a.unpair.fst (eval f c).eval_opt (of_nat code a.unpair.snd) n)) :=
+--begin
+--  funext n, apply roption.ext, intros a,
+--  rw eval_univn_evaln_iff, 
+--  simp[evaln_univn, (>>)], split,
+--  { rintros ⟨s, hs⟩, rcases hs with ⟨e, hs⟩,
+--    have : ∀ x y, evaln (s+1) f c x = some y → (eval f c).eval_opt x = some y,
+--    { intros x y ey, simp[eval_eval_opt], have := evaln_sound ey, exact this },    
+--    have := evaln_inclusion (λ x y e, this x y) _ _ hs,
+--    exact this },
+--  { assume ha, 
+--    have : ∃ s₀, ∀ m a, m < n.unpair.fst.unpair.fst →
+--      eval f c m = option.some a → evaln s₀ f c m = option.some a :=
+--    evaln_comp_dec n.unpair.1.unpair.1, rcases this with ⟨s₀, hs₀⟩,
+--    refine ⟨max n s₀, le_max_left _ _, _⟩, 
+--    have hs₀' : ∀ m a, m < n.unpair.fst.unpair.fst →
+--      (eval f c).eval_opt m = some a → evaln (max n s₀ + 1) f c m = option.some a,
+--    from λ _ _ em ha, evaln_mono (le_trans (le_max_right n _) (nat.le_succ _)) (hs₀ _ _ em (
+--      by { simp at ha, simp[of_option, roption.eq_some_iff] at ha ⊢, exact ha})),
+--    exact evaln_inclusion hs₀' _ _ ha } 
+--end
+
+theorem eval_univn_eq {c f} {g : ℕ → option ℕ} (h : eval f c = (λ x, g x)) : 
+  eval f c.univn = nat.unpaired (λ a n, (evaln a.unpair.fst g (of_nat code a.unpair.snd) n)) :=
+begin
+  unfold_coes at h,
+  funext n, apply roption.ext, intros a,
+  rw eval_univn_evaln_iff, 
+  simp[evaln_univn, (>>)], split,
+  { rintros ⟨s, hs⟩, rcases hs with ⟨e, hs⟩,
+    have : ∀ x y, evaln (s+1) f c x = some y → g x = some y,
+    { intros x y ey, have := evaln_sound ey, simp[h] at this, exact this },    
+    have := evaln_inclusion (λ x y e, this x y) _ _ hs,
+    exact this },
+  { assume ha, 
+    have : ∃ s₀, ∀ m a, m < n.unpair.fst.unpair.fst →
+      g m = option.some a → evaln s₀ f c m = option.some a :=
+    evaln_comp' h n.unpair.1.unpair.1, rcases this with ⟨s₀, hs₀⟩,
+    refine ⟨max n s₀, le_max_left _ _, _⟩, 
+    have hs₀' : ∀ m a, m < n.unpair.fst.unpair.fst →
+      g m = option.some a → evaln (max n s₀ + 1) f c m = option.some a,
+    from λ _ _ em ha, evaln_mono (le_trans (le_max_right n _) (nat.le_succ _)) (hs₀ _ _ em ha),
+    exact evaln_inclusion hs₀' _ _ ha } 
+end
+
+theorem rfind'' {f} : nat.rpartrec f (nat.unpaired (λ a m,
+  (nat.rfind (λ n, (λ m, m = 0) <$> f (nat.mkpair a (n + m)))).map (+ m))) :=
+rpartrec.nat_iff.mp $
+begin
+  simp,
+  have c₀ : primrec (λ (x : (ℕ × ℕ) × ℕ), x.2 + x.1.2) := 
+  primrec.nat_add.comp primrec.snd (primrec.snd.comp primrec.fst),
+  have c₁ : primrec (λ (m : ((ℕ × ℕ) × ℕ) × ℕ), to_bool (m.2 = 0)) :=
+  primrec₂.comp primrec.eq primrec.snd (primrec.const 0),
+  have c₂ : (λ (x : (ℕ × ℕ) × ℕ), f (x.1.1.mkpair (x.2 + x.1.2))) partrec_in f :=
+  rpartrec.refl.comp (primrec₂.mkpair.comp (primrec.fst.comp primrec.fst) $
+    primrec.nat_add.comp primrec.snd (primrec.snd.comp primrec.fst)).to_comp.to_rpart,
+  have := (rpartrec.rfind.trans (c₂.map c₁.to_comp.to_rcomp)).map c₀.to_comp.to_rcomp,
+  simp at this,
+  exact this.comp primrec.unpair.to_comp.to_rcomp
+end
+
+theorem exists_code {f g : ℕ →. ℕ} [D : decidable_pred g.dom] :
+  nat.rpartrec g f → ∃ c, eval (g.eval_opt) c = f := λ h,
+begin
+  induction h,
+  case nat.rpartrec.oracle 
+  { exact ⟨oracle, by { simp[eval], funext n, exact of_to_option (g n) }⟩ },  
+  case nat.rpartrec.zero   { exact ⟨zero, rfl⟩ },
+  case nat.rpartrec.succ   { exact ⟨succ, rfl⟩ },
+  case nat.rpartrec.left   { exact ⟨left, rfl⟩ },
+  case nat.rpartrec.right  { exact ⟨right, rfl⟩ },
+  case nat.rpartrec.pair : f₀ f₁ pf₀ pf₁ hf₀ hf₁
+  { rcases hf₀ with ⟨e₀, rfl⟩, rcases hf₁ with ⟨e₁, rfl⟩,
+    exact ⟨pair e₀ e₁, rfl⟩ },
+  case nat.rpartrec.comp : f₀ f₁ pf₀ pf₁ hf₀ hf₁
+  { rcases hf₀ with ⟨e₀, rfl⟩, rcases hf₁ with ⟨e₁, rfl⟩,
+    exact ⟨comp e₀ e₁, rfl⟩ },
+  case nat.rpartrec.prec : f₀ f₁ pf₀ pf₁ hf₀ hf₁
+  { rcases hf₀ with ⟨e₀, rfl⟩, rcases hf₁ with ⟨e₁, rfl⟩,
+    exact ⟨prec e₀ e₁, rfl⟩ },
+  case nat.rpartrec.rfind : f₀ pf₀ hf₀
+  { rcases hf₀ with ⟨e₀, rfl⟩, 
+    refine ⟨comp (rfind' e₀) (pair nat.rpartrec.code.id zero), _⟩,
+    simp [eval, (<*>), pure, pfun.pure, roption.map_id'],  },
+  case nat.rpartrec.univn : f₀ D pf₀ hf₀
+  { rcases hf₀ with ⟨e₀, h⟩,
+    have : eval g.eval_opt e₀ = λ x, (@pfun.eval_opt _ _ f₀ D) x,
+    { unfold_coes, simp, exact h },
+    have := eval_univn_eq this,
+    refine ⟨e₀.univn, this⟩ },
+end
+
+end nat.rpartrec.code
